Phi_Examples/Linked_List.thy
@@ -2,7 +2,7 @@ theory Linked_List
   imports Phi_Semantics.PhiSem_C
 begin
 
-(*
+
 abbreviation \<open>\<l>\<i>\<n>\<k>_\<l>\<i>\<s>\<t> TY \<equiv> \<s>\<t>\<r>\<u>\<c>\<t> {nxt: \<p>\<t>\<r>, data: TY}\<close>
 
 (*declare [[\<phi>trace_reasoning = 3]]*)
@@ -17,7 +17,8 @@ abbreviation \<open>\<l>\<i>\<n>\<k>_\<l>\<i>\<s>\<t> TY \<equiv> \<s>\<t>\<r>\<
           and \<open>Abstract_Domain T P \<Longrightarrow> Abstract_Domain (Linked_Lst addr T) (\<lambda>x. list_all P x \<and> (x = [] \<longleftrightarrow> addr = 0)) \<close>
           and \<open>Identity_Elements\<^sub>E (Linked_Lst addr T) (\<lambda>l. addr = 0 \<and> l = [])\<close>
           and \<open>Identity_Elements\<^sub>I (Linked_Lst addr T) (\<lambda>l. l = []) (\<lambda>_. addr = 0)\<close>
-        (*and \<open>Transformation_Functor (Linked_Lst addr) (Linked_Lst addr) T U set (\<lambda>_. UNIV) list_all2\<close>
+        (* and \<open> \<c>\<o>\<n>\<d>\<i>\<t>\<i>\<o>\<n> \<t>\<y>\<p>\<e>\<o>\<f> T = \<t>\<y>\<p>\<e>\<o>\<f> U
+            \<Longrightarrow> Transformation_Functor (Linked_Lst addr) (Linked_Lst addr) T U set (\<lambda>_. UNIV) list_all2\<close>
           and \<open>Functional_Transformation_Functor (Linked_Lst addr) (Linked_Lst addr) T U
                                                  set (\<lambda>x. UNIV) (\<lambda>f. list_all) (\<lambda>f P. map f)\<close>*)
 
@@ -82,27 +83,26 @@ proc prepend_llist:
   output \<open>addr' \<Ztypecolon> \<v>\<a>\<l> \<bbbP>\<t>\<r> (\<l>\<i>\<n>\<k>_\<l>\<i>\<s>\<t> (\<t>\<y>\<p>\<e>\<o>\<f> T))\<heavy_comma> v#l \<Ztypecolon> Linked_Lst addr' T \<s>\<u>\<b>\<j> addr'. \<top>\<close>
 \<medium_left_bracket>
   val ret \<leftarrow> calloc1 \<open>\<lbrace> nxt: \<bbbP>\<t>\<r> \<l>\<i>\<n>\<k>_\<l>\<i>\<s>\<t> (\<t>\<y>\<p>\<e>\<o>\<f> T), data: T \<rbrace>\<close> \<semicolon>
-  ret.nxt := addr
-    note [[\<phi>trace_reasoning = 2]]
-    \<semicolon> 
+  ret.nxt := addr \<semicolon> 
   ret.data := v \<semicolon>
   \<m>\<a>\<k>\<e>\<s>(1) \<open>Linked_Lst _ T\<close> \<semicolon>
   ret
 \<medium_right_bracket> .
 
 
+
 proc pop_llist:
-  input  \<open>addr \<Ztypecolon> \<v>\<a>\<l> \<bbbP>\<t>\<r> (\<l>\<i>\<n>\<k>_\<l>\<i>\<s>\<t> TY)\<heavy_comma>
-          l \<Ztypecolon> Linked_Lst addr TY T \<close>
-  output \<open>addr' \<Ztypecolon> \<v>\<a>\<l> \<bbbP>\<t>\<r> (\<l>\<i>\<n>\<k>_\<l>\<i>\<s>\<t> TY)\<heavy_comma>
-          (if l = [] then [] else tl l) \<Ztypecolon> Linked_Lst addr' TY T
+  input  \<open>addr \<Ztypecolon> \<v>\<a>\<l> \<bbbP>\<t>\<r> (\<l>\<i>\<n>\<k>_\<l>\<i>\<s>\<t> (\<t>\<y>\<p>\<e>\<o>\<f> T))\<heavy_comma>
+          l \<Ztypecolon> Linked_Lst addr T \<close>
+  output \<open>addr' \<Ztypecolon> \<v>\<a>\<l> \<bbbP>\<t>\<r> (\<l>\<i>\<n>\<k>_\<l>\<i>\<s>\<t> (\<t>\<y>\<p>\<e>\<o>\<f> T))\<heavy_comma>
+          (if l = [] then [] else tl l) \<Ztypecolon> Linked_Lst addr' T
           \<s>\<u>\<b>\<j> addr'. \<top>\<close>
   is [routine]
 \<medium_left_bracket>
-  if (addr = \<open>0 \<Ztypecolon> \<bbbP>\<t>\<r> (\<l>\<i>\<n>\<k>_\<l>\<i>\<s>\<t> TY)\<close>) \<medium_left_bracket>
+  if (addr = \<open>0 \<Ztypecolon> \<bbbP>\<t>\<r> (\<l>\<i>\<n>\<k>_\<l>\<i>\<s>\<t> (\<t>\<y>\<p>\<e>\<o>\<f> T))\<close>) \<medium_left_bracket>
     return(addr)
   \<medium_right_bracket> \<medium_left_bracket> \<medium_right_bracket> \<semicolon>
-   
+    
   \<t>\<r>\<a>\<n>\<s>\<f>\<o>\<r>\<m>\<s>_\<t>\<o> \<open>\<o>\<p>\<e>\<n>(1)\<close> \<semicolon>
   val ret \<leftarrow> addr.nxt ! \<semicolon>
   mfree (addr) \<semicolon>
@@ -111,10 +111,11 @@ proc pop_llist:
 \<medium_right_bracket> .
 
 
+
 proc nth_llist:
-  input    \<open>addr \<Ztypecolon> \<v>\<a>\<l> \<bbbP>\<t>\<r> (\<l>\<i>\<n>\<k>_\<l>\<i>\<s>\<t> TY)\<heavy_comma> i \<Ztypecolon> \<v>\<a>\<l> \<nat>(\<i>\<n>\<t>)\<heavy_comma> l \<Ztypecolon> Linked_Lst addr TY T\<close>
+  input    \<open>addr \<Ztypecolon> \<v>\<a>\<l> \<bbbP>\<t>\<r> (\<l>\<i>\<n>\<k>_\<l>\<i>\<s>\<t> (\<t>\<y>\<p>\<e>\<o>\<f> T))\<heavy_comma> i \<Ztypecolon> \<v>\<a>\<l> \<nat>(\<i>\<n>\<t>)\<heavy_comma> l \<Ztypecolon> Linked_Lst addr T\<close>
   premises \<open>i < length l\<close>
-  output   \<open>l \<Ztypecolon> Linked_Lst addr TY T\<heavy_comma> l!i \<Ztypecolon> \<v>\<a>\<l> T\<close>
+  output   \<open>l \<Ztypecolon> Linked_Lst addr T\<heavy_comma> l!i \<Ztypecolon> \<v>\<a>\<l> T\<close>
   is [recursive]
   \<medium_left_bracket>
     \<t>\<r>\<a>\<n>\<s>\<f>\<o>\<r>\<m>\<s>_\<t>\<o> \<open>\<o>\<p>\<e>\<n>(1)\<close> \<semicolon> \<comment> \<open>annotation 1: open abstraction\<close>
@@ -123,15 +124,15 @@ proc nth_llist:
     \<medium_right_bracket> \<medium_left_bracket>
         nth_llist (addr.nxt !, i - 1)
     \<medium_right_bracket>
-    \<m>\<a>\<k>\<e>\<s>(1) \<open>Linked_Lst addr TY T\<close> \<comment> \<open>annotation 2: close abstraction\<close>
+    \<m>\<a>\<k>\<e>\<s>(1) \<open>Linked_Lst addr T\<close> \<comment> \<open>annotation 2: close abstraction\<close>
   \<medium_right_bracket> .
 
 thm nth_llist_def
 
 proc hd_llist:
-  input \<open>addr \<Ztypecolon> \<v>\<a>\<l> \<bbbP>\<t>\<r> (\<l>\<i>\<n>\<k>_\<l>\<i>\<s>\<t> TY)\<heavy_comma> l \<Ztypecolon> Linked_Lst addr TY T\<close>
+  input \<open>addr \<Ztypecolon> \<v>\<a>\<l> \<bbbP>\<t>\<r> (\<l>\<i>\<n>\<k>_\<l>\<i>\<s>\<t> (\<t>\<y>\<p>\<e>\<o>\<f> T))\<heavy_comma> l \<Ztypecolon> Linked_Lst addr T\<close>
   premises \<open>l \<noteq> []\<close>
-  output \<open>l \<Ztypecolon> Linked_Lst addr TY T\<heavy_comma>
+  output \<open>l \<Ztypecolon> Linked_Lst addr T\<heavy_comma>
           hd l \<Ztypecolon> \<v>\<a>\<l> T\<close>
 \<medium_left_bracket>
   nth_llist (addr, 0)
@@ -139,9 +140,9 @@ proc hd_llist:
 
 
 proc update_nth_llist:
-  input    \<open>addr \<Ztypecolon> \<v>\<a>\<l> \<bbbP>\<t>\<r> \<s>\<t>\<r>\<u>\<c>\<t> {nxt: \<p>\<t>\<r>, data: TY}\<heavy_comma> i \<Ztypecolon> \<v>\<a>\<l> \<nat>(\<i>\<n>\<t>)\<heavy_comma> y \<Ztypecolon> \<v>\<a>\<l> T\<heavy_comma> l \<Ztypecolon> Linked_Lst addr TY T\<close>
+  input    \<open>addr \<Ztypecolon> \<v>\<a>\<l> \<bbbP>\<t>\<r> \<s>\<t>\<r>\<u>\<c>\<t> {nxt: \<p>\<t>\<r>, data: \<t>\<y>\<p>\<e>\<o>\<f> T}\<heavy_comma> i \<Ztypecolon> \<v>\<a>\<l> \<nat>(\<i>\<n>\<t>)\<heavy_comma> y \<Ztypecolon> \<v>\<a>\<l> T\<heavy_comma> l \<Ztypecolon> Linked_Lst addr T\<close>
   premises \<open>i < length l\<close>
-  output   \<open>l[i := y] \<Ztypecolon> Linked_Lst addr TY T\<close>
+  output   \<open>l[i := y] \<Ztypecolon> Linked_Lst addr T\<close>
   is [recursive]
   \<medium_left_bracket>
     \<t>\<r>\<a>\<n>\<s>\<f>\<o>\<r>\<m>\<s>_\<t>\<o> \<open>\<o>\<p>\<e>\<n>(1)\<close> \<semicolon> \<comment> \<open>annotation 1: open abstraction\<close>
@@ -150,7 +151,7 @@ proc update_nth_llist:
     \<medium_right_bracket> \<medium_left_bracket>
         update_nth_llist (addr.nxt !, i - 1, y)
     \<medium_right_bracket> \<semicolon>
-    \<m>\<a>\<k>\<e>\<s>(1) \<open>Linked_Lst addr TY T\<close>  \<comment> \<open>annotation 2: close abstraction\<close>
+    \<m>\<a>\<k>\<e>\<s>(1) \<open>Linked_Lst addr T\<close>  \<comment> \<open>annotation 2: close abstraction\<close>
   \<medium_right_bracket> .
 
   thm update_nth_llist_def
@@ -158,9 +159,9 @@ proc update_nth_llist:
 end
 
 proc length_of:
-  input    \<open>addr \<Ztypecolon> \<v>\<a>\<l> \<bbbP>\<t>\<r> \<s>\<t>\<r>\<u>\<c>\<t> {nxt: \<p>\<t>\<r>, data: TY}\<heavy_comma> l \<Ztypecolon> Linked_Lst addr TY T\<close>
-  premises \<open>length l < 2 ^ LENGTH(\<i>\<n>\<t>)\<close>
-  output   \<open>length l \<Ztypecolon> \<v>\<a>\<l> \<nat>(\<i>\<n>\<t>)\<heavy_comma> l \<Ztypecolon> Linked_Lst addr TY T\<close>
+  input    \<open>addr \<Ztypecolon> \<v>\<a>\<l> \<bbbP>\<t>\<r> \<s>\<t>\<r>\<u>\<c>\<t> {nxt: \<p>\<t>\<r>, data: TY'}\<heavy_comma> l \<Ztypecolon> Linked_Lst addr T\<close>
+  premises \<open>length l < 2 ^ LENGTH(\<i>\<n>\<t>) \<and> TY' = \<t>\<y>\<p>\<e>\<o>\<f> T\<close>
+  output   \<open>length l \<Ztypecolon> \<v>\<a>\<l> \<nat>(\<i>\<n>\<t>)\<heavy_comma> l \<Ztypecolon> Linked_Lst addr T\<close>
   is [recursive]
   is [routine]
 \<medium_left_bracket>
@@ -169,7 +170,7 @@ proc length_of:
   \<medium_right_bracket> \<medium_left_bracket>
     \<t>\<r>\<a>\<n>\<s>\<f>\<o>\<r>\<m>\<s>_\<t>\<o> \<open>\<o>\<p>\<e>\<n>(1)\<close> \<semicolon>
     val ret \<leftarrow> length_of (addr.nxt !) + 1 \<semicolon>
-    \<m>\<a>\<k>\<e>\<s>(1) \<open>Linked_Lst addr TY T\<close> \<semicolon> (* 1: call the second constructor *)
+    \<m>\<a>\<k>\<e>\<s>(1) \<open>Linked_Lst addr T\<close> \<semicolon> (* 1: call the second constructor *)
     return (ret)
   \<medium_right_bracket>
 \<medium_right_bracket> .
