Phi_System/IDE_CP_App2.thy
@@ -99,14 +99,14 @@ local_setup \<open>
   Phi_Type.add_type {no_auto=true}
         (\<^binding>\<open>Val\<close>, \<^pattern>\<open>Val::VAL \<phi>arg \<Rightarrow> (VAL, ?'a) \<phi> \<Rightarrow> (?'x::one, ?'a) \<phi>\<close>,
          Phi_Type.DIRECT_DEF (Thm.transfer \<^theory> @{thm' Val_def}),
-         \<^here>, Phi_Type.Derivings.empty, [])
+         \<^here>, Phi_Type.Derivings.empty, [], NONE)
    #> snd \<close>
 
 local_setup \<open>
   Phi_Type.add_type {no_auto=true}
         (\<^binding>\<open>Vals\<close>, \<^pattern>\<open>Vals::VAL list \<phi>arg \<Rightarrow> (VAL list, ?'a) \<phi> \<Rightarrow> (?'x::one, ?'a) \<phi>\<close>,
          Phi_Type.DIRECT_DEF (Thm.transfer \<^theory> @{thm' Vals_def}),
-         \<^here>, Phi_Type.Derivings.empty, [])
+         \<^here>, Phi_Type.Derivings.empty, [], NONE)
    #> snd \<close>
 
 let_\<phi>type Val
